IsProvabilityLogic

Foundation/ProvabilityLogic/Arithmetic.lean
@@ -1,32 +1,47 @@
 module
 
 public import Foundation.ProvabilityLogic.Realization
-
-@[expose] public section
 /-!
 # Provability logic of arithmetic theory
 -/
 
-namespace LO.FirstOrder
+@[expose] public section
 
-variable (T U : ArithmeticTheory) [T.Δ₁]
+namespace LO
 
-/-- Provability logic of arithmetic theory-/
-def ArithmeticTheory.ProvabilityLogic : Modal.Logic ℕ := {A | ∀ f : T.StandardRealization, U ⊢ f A}
+open FirstOrder
 
-variable {T U} {A B C : Modal.Formula ℕ}
+namespace Modal
 
-namespace ArithmeticTheory.ProvabilityLogic
+/-- `L` is provability logic of `U` on `T` -/
+abbrev Logic.IsProvabilityLogicOf (L : Modal.Logic ℕ) (T U : ArithmeticTheory) [T.Δ₁] := ∀ A ∈ L, ∀ f : T.StandardRealization, U ⊢ f A
+
+/-- `L` is provability logic of `U` on `T` -/
+abbrev Logic.IsProvabilityLogic (L : Modal.Logic ℕ) : Prop := ∃ T : ArithmeticTheory, ∃ TΔ₁ : T.Δ₁, ∃ U, @Logic.IsProvabilityLogicOf L T U TΔ₁
+
+/-- Provability Logics of `U` on `T` -/
+abbrev ProvabilityLogic := { L : Modal.Logic ℕ // Logic.IsProvabilityLogic L }
+
+end Modal
+
+
+namespace FirstOrder
+
+namespace ArithmeticTheory
+
+variable {T U : ArithmeticTheory} [T.Δ₁] {A : Modal.Formula ℕ}
+
+/-- Provability Logic of `U` on `T` -/
+def ProvabilityLogicOf (T U : ArithmeticTheory) [T.Δ₁] : Modal.ProvabilityLogic := ⟨{A | ∀ f : T.StandardRealization, U ⊢ f A}, ⟨T, inferInstance, U, λ _ h f => h f⟩⟩
 
 @[grind =]
-lemma provable_iff : ProvabilityLogic T U ⊢ A ↔ ∀ f : T.StandardRealization, U ⊢ f A := by
-  simp [Modal.Logic.iff_provable, ArithmeticTheory.ProvabilityLogic]
+lemma ProvabilityLogicOf.provable_iff : (T.ProvabilityLogicOf U).1 ⊢ A ↔ ∀ f : T.StandardRealization, U ⊢ f A := by simp [Modal.Logic.iff_provable, ProvabilityLogicOf]
 
-instance : Entailment.Łukasiewicz (ProvabilityLogic T U) where
+instance : Entailment.Łukasiewicz (T.ProvabilityLogicOf U).1 where
   mdp := by
     rintro A B ⟨hA⟩ ⟨hB⟩;
     constructor;
-    simp only [←Modal.Logic.iff_provable, ProvabilityLogic.provable_iff] at hA hB ⊢;
+    simp only [←Modal.Logic.iff_provable, ProvabilityLogicOf.provable_iff] at hA hB ⊢;
     intro f;
     replace hA : U ⊢ f A ➝ f B := hA f;
     replace hB : U ⊢ f A := hB f;
@@ -34,23 +49,27 @@ instance : Entailment.Łukasiewicz (ProvabilityLogic T U) where
   implyK {_ _} := by
     constructor;
     apply Modal.Logic.iff_provable.mp;
-    apply ProvabilityLogic.provable_iff.mpr;
+    apply ProvabilityLogicOf.provable_iff.mpr;
     simp;
   implyS {_ _ _} := by
     constructor;
     apply Modal.Logic.iff_provable.mp;
-    apply ProvabilityLogic.provable_iff.mpr;
+    apply ProvabilityLogicOf.provable_iff.mpr;
     simp;
   elimContra {_ _} := by
     constructor;
     apply Modal.Logic.iff_provable.mp;
-    apply ProvabilityLogic.provable_iff.mpr;
+    apply ProvabilityLogicOf.provable_iff.mpr;
     intro f;
     dsimp [ProvabilityLogic.Realization.interpret];
     cl_prover;
 
-instance : Entailment.Cl (ProvabilityLogic T U) where
+instance : Entailment.Cl (T.ProvabilityLogicOf U).1 where
 
-end ArithmeticTheory.ProvabilityLogic
+end ArithmeticTheory
 
-end LO.FirstOrder
+end FirstOrder
+
+end LO
+
+end
